

$$(1) \quad \frac{\partial u}{\partial t} + u \cdot \nabla u = -\nabla p / \rho + \nu \nabla^2 u + f \nabla \cdot u = 0$$

$$(2) \quad \frac{u_i^{n+1} - u_i^n}{\Delta t} = \frac{3}{2}T(u_i^n) - \frac{1}{2}T(u_i^{n-1}) - \frac{1}{\rho} \frac{\partial p^{n+1}}{\partial x_i}$$

$$(3) \quad T(u_i^n) = -u_j^n \frac{\partial u_i^n}{\partial x_j} + \nu \frac{\partial^2 u_i^n}{\partial x_j \partial x_j}$$

$$(4) \quad \frac{u_i^* - u_i^n}{\Delta t} = \frac{3}{2}T(u_i^n) - \frac{1}{2}T(u_i^{n-1})$$

$$(5) \quad \nabla^2 p^{n+1} = \frac{\rho \nabla \cdot u^*}{\Delta t}$$

$$(6) \quad \begin{aligned} u_i^{n+1} - u^* &= -\Delta t \frac{\partial p^{n+1}}{\partial x_i} \\ n_{numerical} 1981 \hat{u}(k) &= \frac{1}{k \sqrt{k_1^2 + k_2^2}} \begin{pmatrix} \alpha(k) k k_2 + \beta(k) k_1 k_3 \\ -\alpha(k) k k_1 + \beta(k) k_2 k_3 \\ -\beta(k) (k_1^2 + k_2^2) \end{pmatrix} (7) k = \\ &\frac{\sqrt{k_1^2 + k_2^2 + k_3^2}}{\alpha(k)} = \\ &\sqrt{\frac{E(k)}{4\pi k^2}} \exp i \theta_1 \cos \phi \\ \beta(k) &= \\ &\sqrt{\frac{E(k)}{4\pi k^2}} \exp i \theta_2 \cos \phi \\ &\theta_1 \theta_2 \phi 2\pi E(k) \\ d_{eterministic} 1994 E(k) &= \\ &\frac{q^2}{2A} \frac{k_p}{k_p^{\sigma+1}} \exp \left(-\frac{\sigma}{2} \frac{k}{k_p} \right) (8) \\ p_{redictability} 1997 \hat{f} &= \\ \begin{cases} \frac{\varepsilon}{2E_f} u(k), if 0 < k < k_f \\ 0, otherwise \end{cases} (9) \sim \frac{\varepsilon}{2E_f} = \\ 0.5 \\ i_{inearly} 2003, r_{osales} i_{inear} 2005, \hat{f} &= \\ \frac{\varepsilon}{2E} \hat{u}(10) \frac{\varepsilon}{2E} \\ E = \frac{1}{2} \langle u \cdot u \rangle = \frac{3}{2} u'^2 &= \int_0^{k_{max}} E(k) dk \\ \varepsilon = 2\nu \int_0^{k_{max}} k^2 E(k) dk \\ L = \frac{\pi}{2u'^2} \int_0^{k_{max}} k^{-1} E(k) dk \\ \lambda &= \left(\frac{15\nu u'^2}{\varepsilon} \right)^{1/2} \\ \eta &= \left(\frac{\nu^3}{\varepsilon} \right)^{1/4} \\ T &= \tilde{L}/u' \\ \tau_\eta &= \left(\frac{\nu}{\varepsilon} \right)^{1/2} \\ Re_\lambda &= \frac{u' \lambda}{\nu} \\ a &= \frac{\varepsilon \tilde{L}}{u'^3} \end{aligned}$$

$$\begin{aligned} u &= \\ U_+ &= \\ u' &= \\ U_1 &= \\ 0 &= \\ U_2 &= \\ Sx_1 &= \\ U_3 &= \\ 0 &= \end{aligned}$$

$$(11) \quad \frac{\partial u'}{\partial t} + Sx_1 \frac{\partial u'_i}{\partial x_2} + S\delta_{i2} u'_1 + u'_j \frac{\partial u'_i}{\partial x_j} = -\frac{1}{\rho} \frac{\partial p}{\partial x_i} + \nu \frac{\partial^2 u'_i}{\partial x_j \partial x_j} \frac{\partial u'_i}{\partial x_i} = 0$$